\section{Solutions of Some Differential Equations}
    Consider a differential equation of the form
    \begin{equation*}
        \frac{dy}{dt} = ay - b
    \end{equation*}
    Solution:
    \newline
    First, we perform some basic operations:
    \begin{equation*}
        \frac{dy / dt}{ay - b} = 1
    \end{equation*}
    \begin{equation*}
        \frac{dy / dt}{y - b / a} = a
    \end{equation*}
    Then by the chain rule we get:
    \begin{equation*}
        \frac{d}{dt} \ln |y - b / a| = a
    \end{equation*}
    Then we integrate with respect to t
    \begin{equation*}
        \int \frac{d}{dt} \ln |y - b / a| dt = \int a dt
    \end{equation*}
    \begin{equation*}
        ln |y - b / a| = at + C
    \end{equation*}
    Then through some basic manipulation
    \begin{equation*}
        |y - b / a| = e^{at + C} = e^Ce^{at}
    \end{equation*}
    \begin{equation*}
        y - b / a = \pm e^Ce^{at}
    \end{equation*}
    Let $c = \pm e^C$
    \begin{equation*}
        y - b / a = ce^{at}
    \end{equation*}
    \begin{equation*}
        y = b / a + ce^{at}
    \end{equation*}
    So, $y = b / a + ce^{at}$ is the \textbf{general solution} to $\frac{dy}{dt} = ay - b$. If you have an initial condition $y_o$, that is when $t = 0$, $y = y_o$, we can write $c$ in terms of $y_o$. If we let $c = y_o - b / a$, then when $t = 0$, $y = y_o$.
    \begin{equation*}
        y = b / a + (y_o - b / a)e^{at}
    \end{equation*}